\subsection{Mobius}
$$for n \ge 1 g(n) = \sum_{d|n}f(d)$$ 
$$then f(n) = \sum_{d|n}\mu(d)g(n/d)$$

$$M(n) = \sum_{k=1}^{n}\mu(k), \sum_{n = 1}{x} M([x/n]) = 1$$

\subsection{Catalan}
$$C_n = \sum_{k = 0}^{n - 1} C_kC_{n - 1 - k}$$ 
$$C_n = \frac{1}{n + 1} C_{2n}^{n}$$
$$C_n = C_{2n}^{n} - C_{2n}{n - 1}$$

\subsection{Binomials}
$$\sum_{k = 0}^{n} C_n^k = 2^n$$ 
$$\sum_{m = 0}^{n} C_m^k = C_{n + 1}^{k + 1}$$
$$\sum_{k = 0}^{m} C_{n + k}^k = C_{n + m + 1}^m$$

$$\sum_{k = 0}^{n} (C_n^k)^2 = C_{2n}^n$$
$$\sum_{j = 0}^{k} C_m^j C_{n-m}^{k - j} = C_n^k$$
$$\sum_{j = 0}^{m} C_m^j C_{n-m}^{k - j} = C_{n + 1}^{k + 1}$$

$$\sum_{k = 0}^{n} C_{n - k}^k = F_{n + 1}$$



