\section{Taylor series}
\fbox{\begin{minipage}{0.31\textwidth}
\begin{align*}
& f(x) = \sum_{k=0}^n \frac{f^{(k)}(x_0)}{k!} (x-x_0)^k + o((x-x_0)^n) \\
& \\
&	e^x = \sum_{n = 0}^\infty \frac{x^n}{n!} \hspace{22mm}
	\ln (1 + x) = \sum_{n = 1}^\infty (-1)^{n + 1} \frac{x^n}{n} \\
&	\cos x = \sum_{n=0}^\infty (-1)^n \frac{x^{2n}}{(2n)!} \hspace{5mm}
	\sin x = \sum_{n=0}^\infty (-1)^n \frac{x^{2n + 1}}{(2n + 1)!}
\end{align*}
\end{minipage}}
Generating functions:
\fbox{\begin{minipage}{0.31\textwidth}
\begin{align*}
& [x^i](1 + x)^n = C_{n}^{i} \hspace{18mm}
 [x^i](1 - x)^{-n} = C_{n + i - 1}^{i}\\
&C_{\alpha}^n = \frac{\alpha(\alpha - 1) \dots (\alpha - n + 1)}{n!}\\ 
& \prod_{n \ge 1} (1 - x^n) = \sum_{k = -\infty}^{\infty} (-1)^k x^{\frac{k(3k - 1)}{2}}
\end{align*}
\end{minipage}}
